PurescriptLanguageCstParser/PureScript/CST/Types.lean
@@ -1,32 +1,4 @@
 module
--- prelude
--- public import PurescriptLanguageCstParser.PureScript.CST.Types.PType
--- public import PurescriptLanguageCstParser.PureScript.CST.Types.Expr
-
--- mutual
---   public inductive Expr (error : Type) where
---     | num (val : Int)
---     | add (l r : Expr error)
---     | ifE (cond : Expr error) (thenE elseE : Expr error)
---     deriving Repr, BEq
-
---   private structure Metadata (error : Type) where
---     expr : Expr error
---     meta_ : Metadata error
---     hasError : Option error
---     deriving Repr, BEq
--- end
-
-public inductive Expr (w : Type) : Type where
-  | num (n : Int) : Expr w
-  | add (l : Expr w) (r : Expr w) : Expr w
-  | err (e : w) : Expr w
-
-#print Expr
-
-public inductive ExprF (e s : Type) where
-  | num (val : Int)
-  | add (l r : e)
-  | ifE (cond : s) (thenE elseE : e)
-
-#print ExprF
+prelude
+public import PurescriptLanguageCstParser.PureScript.CST.Types.PType
+public import PurescriptLanguageCstParser.PureScript.CST.Types.Expr
